

ML HW10

Date: 11/05/2025

Week: 10

Author: Alvin B. Lin

Student ID: 112652040

Problem 1: PF-ODE Derivation

1. Consider a forward SDE

$$dx_t = f(x_t, t) dt + g(x_t, t) dW_t,$$

show that the corresponding probability flow ODE is written as

$$dx_t = \left[f(x_t, t) - \frac{\partial}{\partial x} g^2(x_t, t) - \frac{g^2(x_t, t)}{2} \frac{\partial}{\partial x} \log p(x_t, t) \right] dt.$$

Solution:

Before demonstration, we need some setup and lemmas:

Definition 1: Variation

For processes $\phi, \psi : \mathbb{R} \rightarrow \mathbb{R}$, we define the d -variation of ϕ on $[0, T]$ by:

$$[\phi]_d := \lim_{\|\Pi\| \rightarrow 0} \sum_{i=0}^{n-1} |\phi(t_{i+1}) - \phi(t_i)|^d$$

And co-variation is defined as:

$$[\phi, \psi]_d = \sum_{i=0}^{n-1} |\phi(t_{i+1}) - \phi(t_i)| \cdot |\psi(t_{i+1}) - \psi(t_i)|,$$

where for all $n \in \mathbb{Z}^+$, $0 = t_0 \leq t_1 \leq \dots \leq t_n = T$, Π is the partition.

Corollary 1

A continuous process has finite variation must have zero as its quadratic variation.

Proof.

$$0 \leq [\phi]_2 = \lim_{\|\Pi\| \rightarrow 0} \sum_{i=0}^{n-1} |\phi(t_{i+1}) - \phi(t_i)|^2 \leq \limsup_{\|\Pi\| \rightarrow 0} |\phi(t_{i+1}) - \phi(t_i)| \cdot [\phi]_1 = 0 \cdot L = 0$$

Hence $[\phi]_2 = 0$ is proved. □

Corollary 2

A continuous process and a finite variation process have zero as their co-variation.

Proof. Trivial, analogous to the proof to corollary 1. □

Now we consider variations on two main process:

- **Identity map:** $\mathbf{id} : [0, T] \rightarrow \mathbb{R}; t \mapsto t$

$$[\mathbf{id}]_1 = \lim_{\|\Pi\| \rightarrow 0} \sum_{i=0}^{n-1} |\mathbf{id}(t_{i+1}) - \mathbf{id}(t_i)| = \lim_{\|\Pi\| \rightarrow 0} \sum_{i=0}^{n-1} |t_{i+1} - t_i| = \lim_{\|\Pi\| \rightarrow 0} \sum_{i=0}^{n-1} (t_{i+1} - t_i) = T$$

Hence

$$[\mathbf{id}]_1 = T$$

- **Wiener process:** W_t on $[0, T]$.

For an equal length partition Π on $[0, T]$, we have

$$[W_t]_1 = \lim_{\|\Pi\| \rightarrow 0} \sum_{i=0}^{n-1} |W_{t_{i+1}} - W_{t_i}| = \lim_{\|\Pi\| \rightarrow 0} \sum_{i=0}^{n-1} \left| \sqrt{\frac{T}{n}} \varepsilon \right|, \quad \varepsilon \sim \mathcal{N}(0, 1)$$

Since $|\varepsilon|$ is a standard [half-normal distribution](#), meaning that:

$$\mathbb{E}|\varepsilon| = 2 \int_0^{+\infty} \frac{1}{\sqrt{2\pi}} z e^{-\frac{1}{2}z^2} dz = -\frac{2}{\sqrt{2\pi}} e^{-\frac{1}{2}z^2} \Big|_0^{+\infty} = \sqrt{\frac{2}{\pi}}$$

By taking expected value on $[W_t]$, we obtain:

$$\mathbb{E}([W_t]) = \lim_{\|\Pi\| \rightarrow 0} \sum_{i=0}^{n-1} \sqrt{\frac{T}{n}} \mathbb{E}|\varepsilon| = \lim_{n \rightarrow \infty} \left(n \cdot \sqrt{\frac{T}{n}} \cdot \sqrt{\frac{2}{\pi}} \right) = \sqrt{\frac{2T}{\pi}} \lim_{n \rightarrow \infty} \sqrt{n} = +\infty$$

Hence we conclude that

$$[W_t]_1 = +\infty$$

Also, by corollary 1 and 2, we have:

$$[\mathbf{id}]_2 = 0 \quad \text{and} \quad [\mathbf{id}, W_t] = 0$$

Lemma 1: Variation on SDE

For time t and the Browning motion/Wiener process W_t , we have:

$$(dt)^2 = 0; \quad dt dW_t = 0; \quad (dt)^m (dW_t)^n = 0 \quad \text{for } m, n \in \mathbb{Z}^+$$

Proof. By definition,

$$(dt)^2 \equiv d[\mathbf{id}, \mathbf{id}] = d[\mathbf{id}]_2 = d(0) = 0$$

and

$$dt dW_t \equiv d[\mathbf{id}, W_t] = d(0) = 0.$$

Also apply double induction, we can get:

$$(dt)^m (dW_t)^n = 0 \quad \text{for } m, n \in \mathbb{Z}^+$$

□

Lemma 2: Quadratic Variation of Wiener Process

For Wiener Process W_t defined on $[0, T]$, we have:

$$(dW_t)^2 = dt$$

Proof. Recall that for $0 \leq s \leq t \leq T$, we have:

$$W_t - W_s \sim \mathcal{N}(0, t - s) \quad \text{or} \quad W_t - W_s \sim \sqrt{t - s}\varepsilon, \quad \varepsilon \sim \mathcal{N}(0, 1)$$

So, we take the expected value on quadratic variation on W_t , we get:

$$\mathbb{E}([W_t]_2) = \lim_{\|\Pi\| \rightarrow 0} \sum_{i=0}^{n-1} \mathbb{E}[(\sqrt{t_{i+1} - t_i}\varepsilon)^2] = \lim_{\|\Pi\| \rightarrow 0} \sum_{i=0}^{n-1} (t_{i+1} - t_i) \mathbb{E}(\varepsilon^2) \quad (1)$$

Also, by definition of variance:

$$1 = \text{Var}(\varepsilon) = \mathbb{E}(\varepsilon^2) - [\mathbb{E}(\varepsilon)]^2 = \mathbb{E}(\varepsilon^2) - 0^2 \implies \mathbb{E}(\varepsilon^2) = 1 \quad (2)$$

With equation (1) and (2), we obtain:

$$\mathbb{E}([W_t]_2) = \lim_{\|\Pi\| \rightarrow 0} \sum_{i=0}^{n-1} (t_{i+1} - t_i) = T$$

Consider the variance of the quadratic variation on W_t , we have:

$$\text{Var}([W_t]_2) = \lim_{\|\Pi\| \rightarrow 0} \sum_{i=0}^{n-1} \text{Var}((t_{i+1} - t_i)\varepsilon^2) = \lim_{\|\Pi\| \rightarrow 0} \sum_{i=0}^{n-1} (t_{i+1} - t_i)^2 \text{Var}(\varepsilon^2)$$

We will use 4th moment and 2nd moment to solve for $\text{Var}(\varepsilon^2)$:

$$\text{Var}(\varepsilon^2) = \mathbb{E}(\varepsilon^4) - (\mathbb{E}(\varepsilon^2))^2 = 3 - 1^2 = 2$$

Therefore

$$\text{Var}([W_t]_2) = 2 \lim_{\|\Pi\| \rightarrow 0} \sum_{i=0}^{n-1} (t_{i+1} - t_i)^2 = 2[\mathbf{id}]_2 = 0$$

Zero variance implies the random variable is a constant, hence

$$(dW_t)^2 = d[W_t]_2 = dt$$

□

The two lemmas have shown the calculation law in Itô's calculus, one difference is that the general chain rule **does not hold** in Itô's calculus.

$$d\phi(x, t) \neq \frac{\partial \phi}{\partial x} dx + \frac{\partial \phi}{\partial t} dt$$

Theorem 1: Itô's Lemma

for a 1-dimension Itô process $\phi(x, t) \in \mathcal{C}^2(\mathbb{R} \times \mathbb{R})$, we have:

$$d\phi = \frac{\partial \phi}{\partial t} dt + \frac{\partial \phi}{\partial x} dx + \frac{1}{2} \frac{\partial^2 \phi}{\partial x^2} (dx)^2$$

More generally, for an Itô process $\Phi(X, t) \in \mathcal{C}^2(\mathcal{X} \times \mathbb{R})$, $\mathcal{X} \subseteq \mathbb{R}^d$, we have:

$$d\Phi = \frac{\partial \Phi}{\partial t} dt + \nabla \Phi \cdot dX + \frac{1}{2} \sum_{i=1}^d \sum_{k=1}^d \frac{\partial^2 \Phi}{\partial X^i \partial X^k} dX^i dX^k$$

Proof. By **Taylor theorem** and lemma 1 and 2,

$$\begin{aligned} d\phi &= \frac{\partial \phi}{\partial x} dx + \frac{\partial \phi}{\partial t} dt + \frac{1}{2} \frac{\partial^2 \phi}{\partial x^2} (dx)^2 + \frac{1}{2} \frac{\partial^2 \phi}{\partial t^2} (dt)^2 + \frac{\partial^2 \phi}{\partial t \partial x} dt dx + \dots \\ &= \frac{\partial \phi}{\partial x} dx + \frac{\partial \phi}{\partial t} dt + \frac{1}{2} \frac{\partial^2 \phi}{\partial x^2} (dx)^2 + 0 \end{aligned}$$

□

Consider $p(x, t) \in \mathcal{C}^2(\mathbb{R} \times \mathbb{R})$, and let

$$dx_t = f(x, t)dt + g(x, t)dW_t$$

We derive the **Fokker Planck equation** first. For **arbitrary** smooth function with compact support $V(x) \in \mathcal{C}_c^\infty(\mathbb{R})$, then by Itô's lemma,

$$\begin{aligned} dV(x) &= \frac{\partial V}{\partial t} dt + \frac{\partial V}{\partial x} dx + \frac{1}{2} \frac{\partial^2 V}{\partial x^2} (dx)^2 = 0 + \frac{\partial V}{\partial x} (f(x, t)dt + g(x, t)dW_t) + \frac{1}{2} \frac{\partial^2 V}{\partial x^2} g^2(x, t)dt \\ &= \left(\frac{\partial V}{\partial x} f(x, t) + \frac{1}{2} \frac{\partial^2 V}{\partial x^2} g^2(x, t) \right) dt + \frac{\partial V}{\partial x} g(x, t)dW_t \end{aligned}$$

Hence

$$\mathbb{E}(V(x)) = \mathbb{E} \left(\int dV \right) = \mathbb{E} \left(\int \frac{\partial V}{\partial x} f(x, t) + \frac{1}{2} \frac{\partial^2 V}{\partial x^2} g^2(x, t) dt \right) + \cancel{\mathbb{E} \left(\int \frac{\partial V}{\partial x} g(x, t) dW_t \right)} \rightarrow 0$$

Then take the derivative with respect to t ,

$$\begin{aligned} \frac{d}{dt} (\mathbb{E}(V(x))) &= \frac{d}{dt} \left(\mathbb{E} \left(\int \frac{\partial V}{\partial x} f(x, t) + \frac{1}{2} \frac{\partial^2 V}{\partial x^2} g^2(x, t) dt \right) \right) \\ &= \mathbb{E} \left(\frac{d}{dt} \left(\int \frac{\partial V}{\partial x} f(x, t) + \frac{1}{2} \frac{\partial^2 V}{\partial x^2} g^2(x, t) dt \right) \right) \\ &= \mathbb{E} \left(\frac{\partial V}{\partial x} f(x, t) + \frac{1}{2} \frac{\partial^2 V}{\partial x^2} g^2(x, t) \right) \\ &= \int_{\mathbb{R}} \left(\frac{\partial V}{\partial x} f(x, t) + \frac{1}{2} \frac{\partial^2 V}{\partial x^2} g^2(x, t) \right) p(x, t) dx \end{aligned}$$

Recall the original definition of the expected value, which is:

$$\mathbb{E}(V(x)) = \int_{\mathbb{R}} V(x)p(x,t)dx$$

Taking the derivative with respect to t in this expression yields:

$$\frac{d}{dt}(\mathbb{E}(V(x))) = \int_{\mathbb{R}} V(x) \frac{\partial p(x,t)}{\partial t} dx =$$

Two expressions must be equivalent, so:

$$\begin{aligned} \int_{\mathbb{R}} V(x) \frac{\partial p(x,t)}{\partial t} dx &= \int_{\mathbb{R}} \left(\frac{\partial V}{\partial x} f(x,t) + \frac{1}{2} \frac{\partial^2 V}{\partial x^2} g^2(x,t) \right) p(x,t) dx \\ &= \underbrace{\int_{\mathbb{R}} \frac{\partial V}{\partial x} f(x,t) p(x,t) dx}_{(i)} + \frac{1}{2} \underbrace{\int_{\mathbb{R}} \frac{\partial^2 V}{\partial x^2} g^2(x,t) p(x,t) dx}_{(ii)} \end{aligned}$$

Remember that $V(x)$ has compact support, so

$$\lim_{x \rightarrow \pm\infty} V(x) = 0; \quad \lim_{x \rightarrow \pm\infty} \frac{\partial V}{\partial x} = 0$$

We aim to factor out all the $V(x)$, so we do the integration by parts on (i) and (ii).

(i)

$$\int_{\mathbb{R}} \frac{\partial V}{\partial x} f(x,t) p(x,t) dx = \cancel{V(x)f(x,t)p(x,t)} \Big|_{-\infty}^{+\infty} - \int_{\mathbb{R}} V(x) \frac{\partial(f(x,t)p(x,t))}{\partial x} dx$$

(ii)

$$\begin{aligned} \int_{\mathbb{R}} \frac{\partial^2 V}{\partial x^2} g^2(x,t) p(x,t) dx &= \cancel{\frac{\partial V}{\partial x} g^2(x,t) p(x,t)} \Big|_{-\infty}^{+\infty} - \int_{\mathbb{R}} \frac{\partial V}{\partial x} \frac{\partial(g^2(x,t)p(x,t))}{\partial x} dx \\ &= -V(x) \frac{\partial(g^2(x,t)p(x,t))}{\partial x} \Big|_{-\infty}^{+\infty} + \int_{\mathbb{R}} V \frac{\partial^2(g(x,t)p(x,t))}{\partial x^2} dx \end{aligned}$$

Bring back the result in (i) and (ii),

$$\int_{\mathbb{R}} V(x) \frac{\partial p(x,t)}{\partial t} dx = \int_{\mathbb{R}} V(x) \left(-\frac{\partial(f(x,t)p(x,t))}{\partial x} + \frac{1}{2} \frac{\partial^2(g^2(x,t)p(x,t))}{\partial x^2} \right) dx$$

Since our function $V(x)$ is **arbitrary**, so

$$\frac{\partial p(x,t)}{\partial t} = -\frac{\partial(f(x,t)p(x,t))}{\partial x} + \frac{1}{2} \frac{\partial^2(g^2(x,t)p(x,t))}{\partial x^2}, \quad (1)$$

which is the **Fokker Planck equation**.

Theorem 2: Continuity Equation (Physics)

For the density $\rho(x, t)$ of a conserved quantity at position time x and t , $J(x, t)$ be the flux, we have the following relation:

$$\frac{\partial \rho(x, t)}{\partial t} = -\frac{\partial J(x, t)}{\partial x}$$

An intuitive example to the theorem is

“Imagine a single line of people moving into a stadium through a narrow turnstile.”

- State Space (x): The position along the line.
- Density (ρ): The number of people per meter in the line at position x .
- Flux (J): The number of people passing a point x per second.

Does our $p(x, t)$ fit in the equation?

Yes, because $p(x, t)$ is conservative $\left(\int_{\mathbb{R}} p(x, t) dx = 1 \quad \forall t \right)$

So let's assume some $u(x, t)$ s.t. $u(x, t)p(x, t) = J(x, t)$ and satisfy the continuity equation:

$$\frac{\partial p(x, t)}{\partial t} = -\frac{\partial J(x, t)}{\partial x} = -\frac{\partial (u(x, t)p(x, t))}{\partial x} \quad (2)$$

We bring equation (2) to equation (1) to solve for $u(x, t)$:

$$-\frac{\partial (u(x, t)p(x, t))}{\partial x} = \frac{\partial p(x, t)}{\partial t} = -\frac{\partial (f(x, t)p(x, t))}{\partial x} + \frac{\partial}{\partial x} \left(\frac{1}{2} \frac{\partial (g^2(x, t)p(x, t))}{\partial x} \right) \quad (3)$$

Integrate the equation (3) with respect to x , we get:

$$\begin{aligned} -u(x, t)p(x, t) &= -f(x, t)p(x, t) + \frac{1}{2} \frac{\partial (g^2(x, t)p(x, t))}{\partial x} \\ &= -f(x, t)p(x, t) + \frac{1}{2} \frac{\partial g^2(x, t)}{\partial x} p(x, t) + \frac{1}{2} g^2(x, t) \frac{\partial p(x, t)}{\partial x} \\ &= -f(x, t)p(x, t) + \frac{1}{2} \frac{\partial g^2(x, t)}{\partial x} p(x, t) + \frac{1}{2} g^2(x, t) \frac{\partial \log p(x, t)}{\partial x} p(x, t) \end{aligned} \quad (4)$$

We cancel out $p(x, t)$ at both sides, getting:

$$u(x, t) = f(x, t) - \frac{1}{2} \frac{\partial g^2(x, t)}{\partial x} - \frac{g^2(x, t)}{2} \frac{\partial \log p(x, t)}{\partial x}$$

Look back the definition of $u(x, t)$ from the equation (2), we know that $u(x, t)$ stands for the speed of flow, which can also be defined as $\frac{dx_t}{dt}$, so

$$dx_t = u(x_t, t)dt = \left(f(x_t, t) - \frac{1}{2} \frac{\partial g^2(x_t, t)}{\partial x} - \frac{g^2(x_t, t)}{2} \frac{\partial \log p(x_t, t)}{\partial x} \right) dt,$$

which completes the demonstration.